coq/cclc2/clc_soundness.v
@@ -1,7 +1,7 @@
 From mathcomp Require Import ssreflect ssrbool eqtype ssrnat seq.
 From Coq Require Import ssrfun Utf8 Classical.
 Require Import AutosubstSsr ARS 
-  clc_context clc_ast clc_confluence clc_subtype clc_dual clc_typing
+  clc_context clc_ast clc_confluence clc_typing
   clc_weakening clc_substitution clc_inversion clc_validity.
 
 Set Implicit Arguments.
@@ -12,8 +12,8 @@ Theorem subject_step Γ m n A s :
   ok Γ -> Γ ⊢ m : A : s -> m ~> n -> Γ ⊢ n : A : s.
 Proof with eauto using clc_type, step, ok, merge_re_id.
   move=>wf tp. elim: tp n wf=>{Γ m A s}.
-  move=>Γ s l k n o st. inv st.
-  move=>Γ A B s r t i k tyA ihA tyB ihB n o st. inv st.
+  move=>Γ s k n o st. inv st.
+  move=>Γ A B s r t k tyA ihA tyB ihB n o st. inv st.
   { move:(ihA _ o H5)=>tyA'.
     apply: clc_pi...
     destruct s=>//=.
@@ -39,12 +39,11 @@ Proof with eauto using clc_type, step, ok, merge_re_id.
     move:(ihB _ H5)=>tyB'.
     apply: clc_pi... }
   move=>Γ x A s hs n o st. inv st.
-  move=>Γ A B m s r t i k tyP ihP tym ihm n o st.
-  move:(pi_inv tyP)=>[l[tyA[_ tyB]]]. inv st.
+  move=>Γ A B m s r t k tyP ihP tym ihm n o st.
+  move:(pi_inv tyP)=>[tyA[_ tyB]]. inv st.
   { have st : Pi A B s r t ~> Pi A' B s r t...
     move:(ihP _ (re_ok o) st)=>tyP'.
     apply: clc_conv.
-    apply: conv_sub.
     apply: conv1i...
     apply: clc_lam...
     apply: context_conv.
@@ -57,13 +56,13 @@ Proof with eauto using clc_type, step, ok, merge_re_id.
   move:(merge_context_ok_inv mrg o)=>[o1 o2].
   move:(ihm^~ o1)=>{}ihm.
   move:(ihn^~ o2)=>{}ihn. 
-  move:(validity o1 tym)=>[lP tyP]. inv st.
+  move:(validity o1 tym)=>tyP. inv st.
   { move:(lam_inv tyP tym)=>tym1.
     apply: substitution... }
   { move:(ihm _ H2)=>{}ihm.
     apply: clc_app... }
   { move:(ihn _ H2)=>{}ihn.
-    move:(pi_inv tyP)=>[l[tyA[_ tyB]]].
+    move:(pi_inv tyP)=>[tyA[_ tyB]].
     move:(merge_re_re mrg)=>[e1[e2 e3]].
     destruct s.
     { have mrg' : [Γ1] ∘ Γ2 => [Γ].
@@ -72,14 +71,12 @@ Proof with eauto using clc_type, step, ok, merge_re_id.
         rewrite<-pure_re...
       have {}tyB := substitution tyB k mrg' tyn.
       apply: clc_conv.
-      apply: conv_sub.
       apply: conv_beta.
       apply: conv1i...
       apply: clc_app...
       exact: tyB. }
     { have {}tyB := substitutionN tyB tyn.
       apply: clc_conv.
-      apply: conv_sub.
       apply: conv_beta.
       apply: conv1i...
       apply: clc_app...
@@ -90,7 +87,7 @@ Proof with eauto using clc_type, step, ok, merge_re_id.
   move=>Γ k n o st. inv st.
   move=>Γ k n o st. inv st.
   move=>Γ k n o st. inv st.
-  move=>Γ A B s r t i mrg k tyA ihA tyB ihB n o st. inv st.
+  move=>Γ A B s r t mrg k tyA ihA tyB ihB n o st. inv st.
   { move:(ihA _ o H5)=>{ihA}tyA'.
     apply: clc_sigma...
     destruct s; simpl.
@@ -110,18 +107,17 @@ Proof with eauto using clc_type, step, ok, merge_re_id.
     apply: clc_sigma...
     move:(ihB _ (n_ok (re_ok o)) H5)=>//=tyB'.
     apply: clc_sigma... }
-  move=>Γ1 Γ2 Γ A B m n s r t i k1 k2 mrg
+  move=>Γ1 Γ2 Γ A B m n s r t k1 k2 mrg
     tyS ihS tym ihm tyn ihn n0 o st. 
   move:(merge_context_ok_inv mrg o)=>[o1 o2]. 
   move:(merge_re_re mrg)=>[e[e1 e2]].
-  move:(sigma_inv tyS)=>[G1[G2[i0[_[mrg0[tyA tyB]]]]]].
+  move:(sigma_inv tyS)=>[G1[G2[_[mrg0[tyA tyB]]]]].
   move:(merge_re_re mrg0)=>[e3[e4 e5]]. inv st.
   { move:(ihm _ o1 H3)=>{ihm ihS ihn}tym'.
     rewrite<-re_invo in e4.
     rewrite<-re_invo in e5.
     apply:clc_pair...
     apply:clc_conv.
-    apply:conv_sub.
     apply:conv_beta.
     apply:conv1...
     exact:tyn.
@@ -134,7 +130,7 @@ Proof with eauto using clc_type, step, ok, merge_re_id.
     rewrite e5. rewrite<-e2... }
   { move:(ihn _ o2 H3)=>{ihm ihS ihn}tyn'.
     apply:clc_pair... }
-  move=>Γ1 Γ2 Γ m n1 n2 A s t i k mrg
+  move=>Γ1 Γ2 Γ m n1 n2 A s t k mrg
     tym ihm tyA ihA tyn1 ihn1 tyn2 ihn2 n wf st.
   have[wf1 wf2]:=merge_context_ok_inv mrg wf.
   have{}ihm:=ihm _ wf1.
@@ -158,14 +154,12 @@ Proof with eauto using clc_type, step, ok, merge_re_id.
       rewrite<-pure_re... }
     have tymA:=substitution tyA k mrg' tym.
     apply: clc_conv.
-    apply: conv_sub.
     apply: conv_beta.
     apply: conv1i...
     apply: clc_case...
     apply: tymA.
     have tymA:=substitutionN tyA tym.
     apply: clc_conv.
-    apply: conv_sub.
     apply: conv_beta.
     apply: conv1i...
     apply: clc_case...
@@ -186,17 +180,16 @@ Proof with eauto using clc_type, step, ok, merge_re_id.
     apply: clc_letin1... }
   { move:(it_inv tym)=>k.
     by rewrite (merge_pureL mrg k). }
-  move=>Γ1 Γ2 Γ A B C m n s r t k x i leq key mrg 
+  move=>Γ1 Γ2 Γ A B C m n s r t k x leq key mrg
     tym ihm tyC ihC tyn ihn n0 o st.
   move:(merge_context_ok_inv mrg o)=>[o1 o2]. 
-  move:(validity o1 tym)=>[l tyS].
-  move:(sigma_inv tyS)=>[G1[G2[i0[_[mrg0[tyA tyB]]]]]]. 
+  move:(validity o1 tym)=>tyS.
+  move:(sigma_inv tyS)=>[G1[G2[_[mrg0[tyA tyB]]]]].
   move:(merge_re_re mrg)=>[e0[e1 e2]].
   move:(merge_re_re mrg0)=>[e3[e4 e5]].
   inv st.
   { move:(ihm _ o1 H2)=>tym'.
     apply: clc_conv.
-    apply: conv_sub.
     apply: conv_beta.
     apply: conv1i...
     apply: clc_letin2...
@@ -226,10 +219,9 @@ Proof with eauto using clc_type, step, ok, merge_re_id.
     have:=substitution2 tyn k1 k2 mrg2 mrg3 tym1 tym2.
     by asimpl. }
   move=>Γ k n wf st. inv st.
-  move=>Γ i k n o st. inv st.
-  move=>Γ i k n o st. inv st.
-  move=>Γ i k n o st. inv st.
-  move=>Γ A B s i k tyA ihA tyB ihB n o st. inv st.
+  move=>Γ k n o st. inv st.
+  move=>Γ r k n o st. inv st.
+  move=>Γ r A B s k tyA ihA tyB ihB n o st. inv st.
   { constructor...
     destruct s; simpl...
     apply: context_conv.
@@ -246,39 +238,22 @@ Proof with eauto using clc_type, step, ok, merge_re_id.
     rewrite<-pure_re...
     econstructor.
     apply: re_ok... }
-  move=>Γ A B s i k tyA ihA tyB ihB n o st. inv st.
-  { constructor...
-    destruct s; simpl...
-    apply: context_conv.
-    apply: conv1i...
-    rewrite<-re_invo.
-    rewrite<-pure_re...
-    exact: tyB. }
-  { constructor...
-    apply: ihB...
-    destruct s; simpl.
-    econstructor.
-    apply: re_ok...
-    rewrite<-re_invo.
-    rewrite<-pure_re...
-    econstructor.
-    apply: re_ok... }
-  move=>Γ A i k tyA ihA n o st. inv st.
+  move=>Γ r A k tyA ihA n o st. inv st.
   { constructor... }
-  move=>Γ1 Γ2 Γ m n A B C s t i d mrg tyA ihA tyB ihB tym ihm tyn ihn n0 wf st. inv st.
+  move=>Γ1 Γ2 r1 r2 Γ m n A B s t mrg d tyA ihA tym ihm tyn ihn n0 wf st. inv st.
   { have[wf1 wf2]:=merge_context_ok_inv mrg wf.
     econstructor... }
   { have[wf1 wf2]:=merge_context_ok_inv mrg wf.
     econstructor... }
-  move=>Γ A B m s tym ihm n o st. inv st.
-  { constructor... }
-  move=>Γ A B m s tym ihm n o st. inv st.
-  { constructor... }
-  move=>Γ m tym ihm n o st. inv st.
-  { constructor... }
-  move=>Γ m tym ihm n o st. inv st.
-  { constructor... }
-  move=>Γ A B m s i sb tym ihm tyB ihB n o st.
+  move=>Γ r1 r2 A B m s xor tym ihm n o st. inv st.
+  { econstructor... }
+  move=>Γ r1 r2 A B m s xor tym ihm n o st. inv st.
+  { econstructor... }
+  move=>Γ r1 r2 m xor tym ihm n o st. inv st.
+  { econstructor... }
+  move=>Γ r1 r2 m xor tym ihm n o st. inv st.
+  { econstructor... }
+  move=>Γ A B m s sb tym ihm tyB ihB n o st.
   { apply: clc_conv... }
 Qed.
 
